src/sigma_types.mli
@@ -63,7 +63,7 @@ val uncurry_hyps : Names.Id.t -> unit Proofview.tactic
 val curry : Evd.evar_map -> Names.Name.t -> constr ->
             rel_context * constr
 
-val uncurry_call : Environ.env -> Evd.evar_map -> constr ->
+val uncurry_call : Environ.env -> Evd.evar_map -> constr -> constr ->
                    Evd.evar_map * constr * types
 
 val smart_case : Environ.env -> Evd.evar_map ref -> rel_context ->
@@ -75,7 +75,7 @@ val smart_case : Environ.env -> Evd.evar_map ref -> rel_context ->
 module Tactics : sig
   val curry_hyp : Names.Id.t -> unit Proofview.tactic
   val curry : unit Proofview.tactic
-  val uncurry_call : constr -> Names.Id.t -> unit Proofview.tactic
+  val uncurry_call : constr -> constr -> Names.Id.t -> unit Proofview.tactic
 
   val pattern_sigma : Names.Id.t -> unit Proofview.tactic
   val get_signature_pack : Names.Id.t -> Names.Id.t -> unit Proofview.tactic
