test-suite/tabareau_vec.v
@@ -5,6 +5,7 @@ Inductive ℕ (E:Set) : Set :=
 | O : ℕ E
 | S : ℕ E -> ℕ E
 | raise : E -> ℕ E.
+Derive NoConfusion for ℕ.
 
 Arguments O {_}.
 Arguments S {_} _.
@@ -12,6 +13,7 @@ Arguments S {_} _.
 Inductive Vec E (A : Set) : ℕ E -> Set :=
   nil  : Vec E A O
 | cons : forall {n} (x : A) (xs : Vec E A n), Vec E A (S n).
+Derive NoConfusion NoConfusionHom for Vec.
 
 Arguments nil {_ _}.
 Arguments cons {_ _ _} _ _.
@@ -21,17 +23,19 @@ Inductive vector_param E (A : Set) : forall (n : ℕ E), Vec E A n -> Set :=
 | vcons_param : forall (n : ℕ E) (a : A) (v : Vec E A n),
                   vector_param E A n v ->
                   vector_param E A (S n) (cons a v).
-Derive Signature for vector_param.
-
-Derive NoConfusion for ℕ.
-Derive NoConfusion for Vec.
-Derive NoConfusion for vector_param.
-Derive NoConfusionHom for Vec.
-Derive NoConfusionHom for vector_param.
-
-Import Sigma_Notations.
-Open Scope equations_scope.
+Derive Signature NoConfusion NoConfusionHom for vector_param.
 
 Equations param_vector_vcons E (A : Set) (a : A) (n : ℕ E) (v : Vec E A n)
           (X : vector_param E A (S n) (cons a v)) : vector_param E A n v :=
   param_vector_vcons E A _ _ _  (vcons_param _ _ _ X) := X.
+
+Check param_vector_vcons_elim :
+  forall
+    P : forall (E A : Set) (a : A) (n : ℕ E) (v : Vec E A n),
+      vector_param E A (S n) (cons a v) -> vector_param E A n v -> Prop,
+
+    (forall (E A : Set) (a0 : A) (n0 : ℕ E) (v0 : Vec E A n0) (v1 : vector_param E A n0 v0),
+        P E A a0 n0 v0 (vcons_param E A n0 a0 v0 v1) v1) ->
+
+    forall (E A : Set) (a : A) (n : ℕ E) (v : Vec E A n) (X : vector_param E A (S n) (cons a v)),
+      P E A a n v X (param_vector_vcons E A a n v X).
